Core/Linearizability.v
@@ -13,12 +13,12 @@ From Coq Require Import
   Lists.List.
 Import ListNotations.
 
-Definition KConc {T E} (spec : Spec T E) : Spec T E := overObj (spec :> idImpl).
+Definition KConc {E} (spec : Spec E) : Spec E := overObj (spec :> idImpl).
 
-Definition Lin {T E} (spec' : Spec T E) (spec : Spec T E) :=
+Definition Lin {E} (spec' : Spec E) (spec : Spec E) :=
   specRefines spec' (KConc spec).
 
-Definition HBRw_ {T E} (evs evs' : Trace (ThreadEvent T E)) : Prop :=
+Definition HBRw_ {E} (evs evs' : Trace (ThreadEvent E)) : Prop :=
     exists h h' i i' m m',
       i <> i' /\
       evs = h ++ [(i, m); (i', m')] ++ h' /\
@@ -26,23 +26,23 @@ Definition HBRw_ {T E} (evs evs' : Trace (ThreadEvent T E)) : Prop :=
        (exists Ret e v, m' = @RetEv E Ret e v)) /\
       evs' = h ++ [(i', m'); (i, m)] ++ h'.
 
-Definition HBRw {T E} : (Trace (ThreadEvent T E)) -> (Trace (ThreadEvent T E)) -> Prop :=
-  clos_refl_trans (Trace (ThreadEvent T E)) HBRw_.
+Definition HBRw {E} : (Trace (ThreadEvent E)) -> (Trace (ThreadEvent E)) -> Prop :=
+  clos_refl_trans (Trace (ThreadEvent E)) HBRw_.
 
-Inductive AllRetEv {T E} : Trace (ThreadEvent T E) -> Prop :=
+Inductive AllRetEv {E} : Trace (@ThreadEvent E) -> Prop :=
 | NilAllRet : AllRetEv nil
 | ConsAllRet {Ret s i} {m : E Ret} {v : Ret} :
     AllRetEv s ->
     AllRetEv (cons (i, RetEv m v) s).
 
-Inductive AllCallEv {T E} : Trace (ThreadEvent T E) -> Prop :=
+Inductive AllCallEv {E} : Trace (@ThreadEvent E) -> Prop :=
 | NilAllCall : AllCallEv nil
 | ConsCall {Ret s i} {m : E Ret} :
     AllCallEv s ->
     AllCallEv (cons (i, CallEv m) s).
 
-Definition LinRw {T E} : 
-  (Trace (ThreadEvent T E)) -> (Trace (ThreadEvent T E)) -> Prop :=
+Definition LinRw {E} : 
+  (Trace (ThreadEvent E)) -> (Trace (ThreadEvent E)) -> Prop :=
   fun s t => exists sO sP, 
     AllRetEv sP /\ AllCallEv sO /\
     HBRw (s ++ sP) (t ++ sO).
