Util/AtomicUtil.v
@@ -1,0 +1,23 @@
+From LHL.Core Require Import
+  Program
+  Specs.
+
+Record PendingState {E : ESig} := MkPend {
+  ARetTy : Type;
+  AName : ThreadName;
+  ACall : E ARetTy
+}.
+Arguments MkPend {E}.
+Arguments PendingState : clear implicits.
+
+Variant RacyState {E A} :=
+| DefState (s : A) (m : option (PendingState E))
+| UBState.
+Arguments RacyState : clear implicits.
+
+Definition idleSt {E A} (s : A) : RacyState E A :=
+  DefState s None.
+Definition pendSt {E A} (s : A) (i : ThreadName) (m : E A) :=
+  DefState s (Some (MkPend _ i m)).
+Definition ubSt {E A} : RacyState E A :=
+  UBState.
