Util/TransUtil.v
@@ -222,6 +222,25 @@ Lemma help10 :
 firstorder.
 Qed.
 
+Lemma eqbT : forall n, eqb n n = true.
+intros.
+induction n; easy.
+Qed.
+
+Axiom excluded_middle : forall P, P \/ ~P.
+
+Lemma eqbF : forall n m, n <> m -> n =? m = false.
+fix rec 1.
+intros.
+destruct n, m.
+congruence.
+reflexivity.
+reflexivity.
+simpl.
+apply rec.
+congruence.
+Qed.
+
 Lemma unprojPointTrace {I A} {ieq : I -> I -> bool} :
   (forall i, ieq i i = true) ->
   (exists i : I, True) ->
